\documentclass[12pt]{article}
\usepackage{graphicx,tikz,tikz-network,tkz-euclide}
\usepackage{amsfonts,amsmath,amssymb}
\title{Math Club Sixth Week}
\usetikzlibrary {positioning}
%\usepackage {xcolor}
\definecolor {processblue}{cmyk}{0.96,0,0,0}

\parindent 0pt
\date{October 2024}

\newcounter{problem}
\setcounter{problem}{0} % Initialize the counter at 0
\newcounter{sectionB}
\setcounter{sectionB}{0}

\newcommand{\problem}[1]{
    \stepcounter{problem}
    \noindent\textbf{Problem $A\theproblem$:} #1
     \\ % Add space after the problem statement
}
\newcommand{\problemB}[1]{
    \stepcounter{sectionB} % Increment the counter for Section B
    \noindent\textbf{Problem $B\thesectionB$:} #1
    \\[1em] % Space after the problem statement
}
\newcommand{\multChoice}[5]{
    \begin{tabular}{l @{\hskip 1.5cm} l @{\hskip 1.5cm} l @{\hskip 1.5cm} l @{\hskip 1.5cm} l}
    A. #1 & B. #2 & C. #3 & D. #4 & E. #5
\end{tabular}

}
\newcommand{\solution}[1]{
    \vspace{1em} % Add space before the solution
    \noindent\textbf{Solution:} #1
     % Add space after the solution
}

\setlength{\baselineskip}{5\baselineskip}


\usetikzlibrary {positioning}
%\usepackage {xcolor}
\definecolor {processblue}{cmyk}{0.96,0,0,0}
\newcommand{\myVertex}[3]{
    \Vertex[x=#1,y=#2,size=0.5,label=$#3$,position=90,fontscale=2,style={color=red}]{#3}
}
\newcommand{\simpleVertex}[3]{
    \Vertex[x=#1,y=#2,size=0.5,position=180,fontscale=2,style={color=red}]{#3}
}
\newcommand{\invisibleVertex}[3]{
    \Vertex[x=#1,y=#2,size=0.5,opacity =0,position=180,fontscale=2,style={color=white}]{#3}
}

\begin{document}
\sloppy
\maketitle

\section*{AMATYC problems}

\begin{problem}[G][2][AMATYC Fall 2007/3]
   % Geometry
   A square is covered by a design made up of four identical rectangles
   surrounding a central square, as shown above. If the area of the
   central square is 4/9 of the area of the entire design, find the ratio of the length of a rectangle to the side of the central square. 
   \begin{center}
      \begin{tikzpicture}
          \tkzDefPoints{0/0/A_1, 3/0/B_1, 3/3/C_1, 0/3/D_1}
          \tkzDefPoints{0.5/0/A_2, 3/0.5/B_2, 2.5/3/C_2, 0/2.5/D_2}
          \tkzDefPoints{0.5/0.5/A_3, 2.5/0.5/B_3, 2.5/2.5/C_3, 0.5/2.5/D_3}
            
          \tkzDrawSegments(A_1,B_1 B_1,C_1 C_1,D_1 D_1,A_1)
          \tkzDrawSegments(D_3,A_2 A_3,B_2 B_3,C_2 C_3,D_2)
          
          \node at (-6,3) [left] {A. $5/4$};
          \node at (-3,3) [left] {B. $4/3$};
          \node at (-6,1.8) [left] {C. $7/5$};
          \node at (-3,1.8) [left] {D. $3/2$};
          \node at (-4.5,0.6) [left] {E. $8/5$};
      \end{tikzpicture}
      \end{center}
\end{problem}

\begin{solution}
      A. $5/4$ \\
      Let $x$ be the side length of the inner square, the $y$ be the side length of the outer square, and $z$ be the width (the shorter side) of each rectangle. Note that we are looking for the ratio between $x+z$ and $x$. Also, obverse that
      \begin{align}
         z=\frac{1}{2}(y-x)
      \end{align}
      Since $A_{in}/A_{out}=4/9$, we can say 
      \begin{align} \setcounter{equation}{1}
         \frac{x^2}{y^2} = \frac{4}{9} \: \Rightarrow \: x = \frac{2}{3}y
      \end{align}
      We can then plug this into (1) to get 
      \begin{align*}
         z = \frac{1}{2}(y-\frac{2}{3}y) = \frac{1}{6}y
      \end{align*}
      Now we have what we are looking for: 
      \begin{align*}
         \frac{x+z}{x} &= \frac{(\frac{2}{3}+\frac{1}{6})y}{\frac{2}{3}y} \\
         &= \boxed{\frac{5}{4}}
      \end{align*}
\end{solution}

\begin{problem}[N][3][AMATYC Spring 2017/4]
   % Divisibility ^ MinMax ^ Student Math League
   If cars hold 5 passengers and charge for \$29 a trip to the airport, and vans hold 7 passengers and charge \$41, find the minimum cost to transport 49 people to the airport. \\
\end{problem}
\multChoice{\$290}{\$285}{\$287}{\$280}{\$282}


\begin{solution}[B. \$285]
   Let integers $c$ and $v$ represent the number of cars and vans used respectively, and let $B$ represent the cost we are trying to minimize. Then
   \begin{align} \setcounter{equation}{0}
       5c + 7v &= 49 \\
       29c + 41v &= B
   \end{align}
   Rewriting (1) gives us
   \begin{align*}
       5c &= 49 - 7v \\
       &= 7(7-7v)
   \end{align*}
   which tells us that $7 \mid 5c$. Since $7 \nmid 5$, we can say that $7 \mid c$. But (1) makes it obvious that $c < 10$, so we must conclude that $c=7$. Plugging this back into (1) gives us $v=2$. This appears to be the only solution in which $c$ and $v$ are both positive and integers so we are reasonable to conclude that these values give us the correct answer. \\[5pt] Finally, we use (2) to evaluate the minimum cost.
   \begin{align*}
       29(7) + 41(2) = 203 + 82 = \boxed{285}
   \end{align*}
\end{solution}

\begin{problem}[A][3][AMATYC Fall 2008/8]
   % Algebra ^ Trig ^ Student Math League
   $$ \csc^{-1}{\left(\frac{5}{4}\right)}+\sec^{-1}{\left(\frac{5}{4}\right)}+\cot^{-1}{\left(\frac{5}{4}\right)}+\cot^{-1}{\left(\frac{4}{5}\right)}$$
\end{problem}
\multChoice{$2\pi$}{$\pi$}{$\pi/2$}{$\pi/3$}{$\pi/4$}


\begin{solution}[B]
   First, let's make this problem a bit more comfortable for everyone by remembering that $\sin{\theta}=1/\csc{\theta}$, $\cos{\theta}=1/\sec{\theta}$, and $\tan{\theta}=1/\cot{\theta}$. This allows us to rewrite the expression as 
   \begin{align*}
      \sin^{-1}{\left(\frac{4}{5}\right)}+\cos^{-1}{\left(\frac{4}{5}\right)}+\tan^{-1}{\left(\frac{4}{5}\right)}+\tan^{-1}{\left(\frac{5}{4}\right)}
   \end{align*}
   Our main tool here will be the identity
   \begin{align} \setcounter{equation}{0}
      \sin{(\frac{\pi}{2}-x)}=\cos{(x)}
   \end{align}
   Now, let $\theta_1 = \sin^{-1}{\left(\frac{4}{5}\right)}$ and $\theta_2 = \cos^{-1}{\left(\frac{4}{5}\right)}$ and note that $-\frac{\pi}{2} \leq \theta_1 \leq \frac{\pi}{2}$ and $0 \leq \theta_2 \leq \pi$.
   Since
   \begin{align*}
      \sin{\theta_1} = \frac{4}{5}, \: \cos{\theta_2} = \frac{4}{5} \: \Rightarrow \: \sin{\theta_1} = \cos{\theta_2}
   \end{align*}
   we can use (1) to conclude that $\theta_1 = \frac{\pi}{2} - \theta_2$. Thus,
   \begin{align*}
      \sin^{-1}{\left(\frac{4}{5}\right)}+\cos^{-1}{\left(\frac{4}{5}\right)} &= \theta_1 + \theta_2 \\
      &= (\frac{\pi}{2} - \theta_2) + \theta_2 \\
      &= \frac{\pi}{2}
   \end{align*}
   A similar process can be used to show that 
   \begin{align*}
      \tan^{-1}{\left(\frac{4}{5}\right)}+\tan^{-1}{\left(\frac{5}{4}\right)} = \frac{\pi}{2}
   \end{align*}
   Finally, adding these together, we find that 
   \begin{align*}
      \sin^{-1}{\left(\frac{4}{5}\right)}+\cos^{-1}{\left(\frac{4}{5}\right)}+\tan^{-1}{\left(\frac{4}{5}\right)}+\tan^{-1}{\left(\frac{5}{4}\right)} &= \frac{\pi}{2} + \frac{\pi}{2} \\
      &= \boxed{\pi}
\end{align*}
\end{solution}

\newpage

\begin{problem}[N][3][AMATYC Fall 2004/4]
   % System of Equations ^ Student Math League
   Lucia is not yet 80 years old. Each of her sons has as many sons as brothers. The combined number of Luciaâ€™s sons and grandsons equals her age, and her oldest grandson is 29. How old is Lucia? (Assume you must be 17 or older to have children.) 
    
\end{problem}

\begin{solution}
   64 \\
   Let $L$ represent Lucia's age. The problem tells us that she is younger than 80 and that her oldest grandson is 29. This means she has a son that is at least 46 ($29+17$) and that Lucia herself is at least 63. So $63 \leq L \leq 79$. \\[5pt]
   We also know that if Lucia has $x$ sons, then each of those sons has $x-1$ brothers (since you would not count yourself as a brother). As a result, all $x$ sons raise $x-1$ of their own sons for a total of $x(x-1)$ grandsons. Lucia's age, then, is $L = x + x(x-1) = x^2$. \\[5pt]
   Since the only perfect square between 63 and 79 is $8^2$, we conclude $L=\boxed{64}$.
\end{solution}

\vskip 1cm

\begin{problem}[N][5][AMATYC Spring 2017/7]
   % Algebra ^ Inequalities ^ Student Math League
   Let $a$ and $b$ be positive integers such that $(a,b)$ is a solution to
   $$\sqrt[3]{a+4\sqrt{b}} + \sqrt[3]{a-4\sqrt{b}} = 3$$
   Find the smallest possible value of $a+b$.
   \multChoice{14}{18}{22}{26}{30}
\end{problem}

\vskip 0.5cm

\begin{solution}[A]
   We are starting with 
   \begin{align} \setcounter{equation}{0}
      \sqrt[3]{a+4\sqrt{b}} + \sqrt[3]{a-4\sqrt{b}} = 3
   \end{align}
   The cube roots obviously make this equation ugly, and we are tempted to cube both sides, hoping it works out. Let's see if this is a productive route. Note that
   \begin{align} 
      (x+y)^3 &= x^3 + 3x^2y + 3xy^2 + y^3 \notag \\
      &= x^3 + 3xy(x+y) + y^3
   \end{align}
   If we let $x=\sqrt[3]{a+4\sqrt{b}}$ and $y=\sqrt[3]{a-4\sqrt{b}}$ and plug these into the terms of (2), there are quite a few nice simplifications here, especially making use of (1), which tell us that $x+y=3$.
   \begin{align}
      (x+y)^3 &= x^3 + 3xy(x+y) + y^3 \notag \\
      &= \left(a+4\sqrt{b}\right) + 3\left[\sqrt[3]{\left(a+4\sqrt{b}\right)\left(a-4\sqrt{b}\right)}\right]\!(3) + \left(a-4\sqrt{b}\right) \notag \\
      &= 2a + 9\sqrt[3]{a^2-16b}
   \end{align}
   This seems promising. We now know that cubing both sides of (1) gives us (3) on the left and 27 on the right.
   \begin{align}
      \left(\sqrt[3]{a+4\sqrt{b}} + \sqrt[3]{a-4\sqrt{b}}\right)^3 &= 3^3 \notag \\
      2a + 9\sqrt[3]{a^2-16b} &= 27
   \end{align}
   Since $a\in\mathbb{Z}$, we know $\sqrt[3]{a^2-16b}\in\mathbb{Z}$ as well (since the terms in (4) sum to an integer). From this it follows that $2a=27-9k=9(3-k)$, so $9\mid2a$, which further implies $9\mid a$.
   \\[5pt]
   So $a=9, 18, 27,\dots$ (recall that $a>0$). Notice that depending on the value of $a$, the cube root could be positive or negative. Let's consider two cases: $a = 9$ and $a \geq 18$.
   \\[5pt]
   If $a = 9$, we have
   \begin{align*}
      2(9) + 9\sqrt[3]{(9)^2-16b} &= 27 \\
      \sqrt[3]{81-16b} &= 1 \\
      16b &= 80 \\
      b &= 5
   \end{align*}
   So a potential solution with $a=9$ and $b=5$ for $a+b=14$. Since $b$ cannot be negative, we can quickly see that in the $a \geq 18$ case, $a+b\geq18>14$. This means $a+b=9+5=\boxed{14}$ must be our solution.
\end{solution}

\begin{problem}[A][5][AMATYC Spring 2006]
   % Bezout's Identity ^ Algebra ^ Student Math League
   Which of the following imply that the real number $x$ must be rational? \hspace{2.7em} \\ 
   $$\text{(I): } x^5,x^7 \text{ are both rationals}$$
   $$\text{(II): } x^6,x^8 \text{ are both rationals}$$
   $$\text{(III): } x^5,x^8 \text{ are both rationals}$$
   \multChoice{I,II}{I,III}{II,III}{III only}{none of these}
\end{problem}

\begin{solution}[B]
   First note that $a,b \in \mathbb{Q}$ means that  $a/b$ and $ab$ are also rationals \\
    Let's analyze (I), (II) and (III) to see what conditions are sufficient for $x$ to be a rational number.
    \begin{align*}
        (I) &\Rightarrow (x^7)^2 = x^{14} \in \mathbb{Q} \\
        &\Rightarrow (x^5)^3 = x^{15} \in \mathbb{Q} \\
        &\Rightarrow \frac{x^{15}}{x^{14}} = x \in \mathbb{Q}
    \end{align*}
    Then (I) is sufficient.
    \begin{align*}
        (III) &\Rightarrow  (x^8)^2 = x^{16} \in \mathbb{Q} \\
        &\Rightarrow (x^5)^3 = x^{15} \in \mathbb{Q} \\
        &\Rightarrow \frac{x^{16}}{x^{15}} = x \in \mathbb{Q}
    \end{align*}
    Then (III) is also sufficient. \\
    Now let's show that (II) it is not by letting $x=\sqrt{2}$.\\ 
Clearly $x^6,x^8 \in \mathbb{Q}$ but $x \notin \mathbb{Q}$. \\
Then our answer is $\boxed{B}$ 
\vskip 0.2cm
In general if we have that $x^n,x^m \in \mathbb{Q}$ with $n,m \in \mathbb{Z}^{+} $, then we have $x \in \mathbb{Q}$ only when there exist $u,v \in \mathbb{Z}$ such that $nu+mv=1$, this happens if and only if $\gcd(n,m)=1$ , the reader may look at Bezout's Theorem to understand why. 
\end{solution}

\begin{problem}[A][6][AMATYC Spring 2010/14]
   % Induction ^ Student Math League
   For a function $f(x)$, define $f^2(x)=f(f((x))$ , $f^3(x)=f(f(f(x)))$, and so on. For the function 
    $$f(x) = \sqrt{\frac{x^2+1}{x^2-1}} \text{ where } x \in (-\infty,-1) \cup (1,\infty) $$
    We have $f^{2010}(x)$ to be: \\
    \multChoice{$x$}{$|x|$}{$x^2$}{$1/x$}{$1/x^2$}
\end{problem}

\begin{solution}[B]
      First let's find $f^2(x) = f(f(x))$:
      \begin{align*}
         f(f(x)) &= \sqrt{ \frac{ (x^2+1)/(x^2-1)+1 } { (x^2+1)/(x^2-1) -1} } \\
         &= \sqrt{ \frac{ (2x^2)/(x^2-1) }{ 2/(x^2-1) } } \\
         &= \sqrt{x^2} = |x|
      \end{align*}
      Note that for any $\varphi>1$ ,  $f^2(\varphi) = |\varphi| = \varphi$
      Since $f(x)>1$, we have \\
      \begin{align*}
         f^3(x)=f^2(f(x)) = f(x) \\
         f^4(x) = f(f^3(x)) = f(f(x)) = f^2(x) = |x|
      \end{align*}
      Since $f^n$ alternates between these two values, we see that
      \begin{align*}
         f^{2010}(x) &= f^2(f^{2008}(x)) = f^{2008}(x)\\
         &= f^2(f^{2006}(x)) = f^{2006}(x) \\
         &= \ldots \\
         &= f^2(f^2(x)) = f^2(x) \\
         &= \boxed{|x|}
      \end{align*}
      It is also possible to prove by induction that \\
      $f^{2n+1}(x) = f(x)$ and $f^{2n}(x)=|x|$ for any $n \in \mathbb{Z}^{+}$.
\end{solution}

\newpage

\section*{Calculus Problems}

\begin{problem}[R][4][BMT 2021/4]
   % Integrals ^ BMT
   Compute the area of the region of points satisfying the inequalities 
\[ y \leq 4 - \frac{x^2}{9}, \quad y \geq \frac{x^2}{9} - 4, \quad x \leq 4 - \frac{y^2}{9}, \quad \text{and} \quad x \geq \frac{y^2}{9} - 4. \]
\end{problem}

\vspace{-1.5cm}

\begin{solution}[52]
   The region enclosed by these parabolas is a square with extra parabola lumps of equal size, with vertices at the intersections of the parabolas at \((\pm 3, \pm 3)\). The area of a parabola lump is \(\int_{-3}^{3} \left( \left(4 - \frac{x^2}{9}\right) - 3 \right) \, dx = 4\), and the area of the square is \(6^2 = 36\), so the area of the region is $36 + 4 \cdot 4 = \boxed{52}$.
\end{solution}

\vspace{1cm}

\begin{problem}[R][6][BMT 2021/6]
   % Induction ^ Limits ^ BMT
   Let \(x_1 = -4\), and for \(n \geq 1\) define \(x_{n+1} = -4^{x_n}\). Similarly, define $f_n$ as \(f_1(x) = \sin(\arccos(x))\), and for \(n \geq 1\): \(f_{n+1}(x) = f_1(f_n(x))\). Compute 
    \[
    \lim_{n \to \infty} f_n(2^{2^n}).
    \]
    You may assume that this limit exists.
\end{problem}

\begin{solution}[$\frac{1}{\sqrt{2}}$]
   We start by finding \(\lim_{n \to \infty} x_n\). Say that this limit evaluates to \(x\). We are given that
\[
x_{n+1} = -4^{x_n}.
\]
Taking the limit of both sides as \(n \to \infty\),
\[
x = -4^x.
\]
Drawing the graphs for these functions, we observe that they intersect only once. Hence, there is only one solution for \(x\). After some guess and check, we find that \(x = -\frac{1}{2}\) works and must be the unique solution. \\[10pt]
We now evaluate the desired limit:
\[
\lim_{n \to \infty} f_n(2^{x_n}) = \lim_{n \to \infty} f_n(2^x) = \lim_{n \to \infty} f_n\left(\frac{1}{\sqrt{2}}\right).
\]
Note that \(f_1\left(\frac{1}{\sqrt{2}}\right) = \frac{1}{\sqrt{2}}\), so it can be shown through induction that \(f_n\left(\frac{1}{\sqrt{2}}\right) = \frac{1}{\sqrt{2}}\) for all integers \(n\). \\[10pt]
Therefore, we have
\[
\lim_{n \to \infty} f_n(2^{x_n}) = \boxed{\frac{1}{\sqrt{2}}}.
\]
\end{solution}

\vspace{1cm}

\begin{problem}[R][5][BMT 2021/7]
   % Derivatives ^ BMT
   Let \( c(x) \) be a function defined on the interval \(1 \leq x \leq 2\). Let \(c^{-1}(x)\) be the inverse of \(c(x)\). If
   \[c(x) = \frac{e^x + e^{-2x}}{2}\]
   Compute
   \[ \int_{c(1)}^{c(2)} c^{-1}(x) \, dx. \]
\end{problem}

\vspace{-1.2cm}

\begin{solution}[ $\frac{1}{2}e^2+\frac{5}{4}e^{-4}-\frac{3}{4}e^{-2}$]
   We don't really want to figure out what $c^{-1}(x)$ is, so instead, we'll opt for a clever u-substitution.
\begin{align*}
    u = c^{-1}(x) \iff x &= c(u) \\
    dx &= c'(u)du
\end{align*}
Also, we change the bounds:
\begin{align*}
    x = c(2) &\rightarrow u = 2 \\
    x = c(1) &\rightarrow u = 1
\end{align*}
So now we have
\begin{align*}
    \int_{c(1)}^{c(2)} c^{-1}(x) \, dx = \int_{1}^{2} u \, c'(u) \, du
\end{align*}
which can be computed fairly easily using integration by parts.
\begin{align*}
    \int_{1}^{2} u \, c'(u) \, du &= u\,c(u) \bigg\rvert_{1}^{2} - \int_{1}^{2} c(u) \, du \\
    &= \frac{1}{2}(u)(e^u + e^{-2u}) - \frac{1}{2}(e^u - \frac{1}{2}e^{-2u}) \bigg\rvert_{1}^{2} \\
    &= \boxed{\frac{1}{2}e^2+\frac{5}{4}e^{-4}-\frac{3}{4}e^{-2}}
\end{align*}
\end{solution}

\end{document}